src/study/Nemonuri.Study.CSharpSyntaxRewriter2.Modifier2/Nemonuri.StratifiedNodes.Forall.Children.fst
@@ -18,35 +18,141 @@ let for_all_continue_predicate (t:eqtype)
   =
   fun n v -> v
 
-(*
-let for_all_select_and_aggregate_from_children_internal #t (parent:N.node t) 
-  (parent_value: t2)
-  (node_predicate:N.node t -> Tot bool)
-*)
 
-(*
-let for_all_select_and_aggregate_from_children #t
+let for_all_self_and_children #t
   (parent:N.node t) 
-  (node_predicate:N.node t -> Tot bool)
-  (ancestors:C.head_given_ancestor_list parent)
+  (node_predicate:C.ancestor_list_given_selector t bool)
+  (ancestors:C.next_head_given_ancestor_list parent)
   : Tot bool =
-  let selector : (C.ancestor_list_given_selector_for_child t bool parent) = (
-    C.to_ancestor_list_given_selector_for_child t bool
-      parent node_predicate
+  let node_predicate_for_child : (C.ancestor_list_given_selector_for_child t bool parent) = (
+    C.to_ancestor_list_given_selector_for_child t bool parent node_predicate
   ) in
-  let parent_value = node_predicate parent in
   C.select_and_aggregate_from_children 
-    parent parent_value selector
+    parent node_predicate node_predicate_for_child
     for_all_aggregator
     for_all_aggregator
     (Common.aggregated_identity bool)
     (for_all_continue_predicate t)
     ancestors
-*)
-//---|
+    (N.get_children parent)
+    None
 
 //--- propositions ---
+
+let node1_satisfies_for_all_self_and_children_entails_node2_satisfies_predicate #t
+  (node1:N.node t) 
+  (node_predicate:C.ancestor_list_given_selector t bool)
+  (ancestors1:C.next_head_given_ancestor_list node1)
+  (node2:N.node t)
+  (ancestors2:C.next_head_given_ancestor_list node2)
+  : prop =
+  ((for_all_self_and_children node1 node_predicate ancestors1) ==> 
+   (node_predicate node2 ancestors2))
+
+let node_satisfies_for_all_self_and_children_entails_all_children_nodes_satisfy_predicate #t
+  (node:N.node t)
+  (node_predicate:C.ancestor_list_given_selector t bool)
+  (ancestors:C.next_head_given_ancestor_list node)
+  : prop =
+  forall child_node. 
+  (C.is_parent node child_node) ==>
+  (node1_satisfies_for_all_self_and_children_entails_node2_satisfies_predicate 
+    node node_predicate ancestors
+    child_node (C.concatenate_as_ancestor_list node ancestors)
+  )
+
 //---|
 
 //--- proof ---
+
+let lemma1 #t
+  (parent:N.node t) 
+  (node_predicate:C.ancestor_list_given_selector t bool)
+  (ancestors:C.next_head_given_ancestor_list parent)
+  : Lemma
+    (requires (N.is_leaf parent))
+    (ensures 
+      node_satisfies_for_all_self_and_children_entails_all_children_nodes_satisfy_predicate
+        parent node_predicate ancestors
+    )
+  =
+  ()
+
+
+
+(*
+let lemma4 #t
+  (parent:N.node t) 
+  (node_predicate:C.ancestor_list_given_selector t bool)
+  (prepending:N.node t)
+  : Lemma
+    (requires 
+      (N.is_leaf parent) /\ 
+      (for_all_self_and_children parent node_predicate []) /\ 
+      (N.is_leaf prepending) /\
+      ( let parent2 = D.prepend_child prepending parent in
+        let prepended = N.get_child_at parent2 0 in
+        node_predicate prepended [parent2] )
+    )
+    (ensures (
+      let parent2 = D.prepend_child prepending parent in
+      for_all_self_and_children parent2 node_predicate []
+    ))
+  =
+  let parent2 = D.prepend_child prepending parent in
+  let prepended = N.get_child_at parent2 0 in
+  assert (N.get_children_length parent2 = 1);
+  assert (N.get_level parent2 = 2)
+*)
+
+(*
+let lemma3 #t
+  (parent:N.node t) 
+  (node_predicate:C.ancestor_list_given_selector t bool)
+  (prepending:N.node t)
+  : Lemma
+    (requires 
+      (for_all_self_and_children parent node_predicate []) /\ 
+      ( let parent2 = D.prepend_child prepending parent in
+        let prepended = N.get_child_at parent2 0 in
+        node_predicate prepended [parent2] )
+    )
+    (ensures (
+      let parent2 = D.prepend_child prepending parent in
+      for_all_self_and_children parent2 node_predicate []
+    ))
+  =
+  ()
+*)
+
+(*
+let lemma3 #t
+  (parent:N.node t) 
+  (node_predicate:C.ancestor_list_given_selector t bool)
+  //(ancestors:C.next_head_given_ancestor_list parent)
+  (prepending:N.node t)
+  : Lemma
+    (requires for_all_self_and_children 
+      (D.prepend_child prepending parent) node_predicate []
+    )
+    (ensures for_all_self_and_children 
+      parent node_predicate []
+    )
+  =
+  ()
+*)
+
+(*
+let lemma2 #t
+  (parent:N.node t) 
+  (node_predicate:C.ancestor_list_given_selector t bool)
+  : Lemma 
+    (ensures 
+      node_satisfies_for_all_self_and_children_entails_all_children_nodes_satisfy_predicate
+        parent node_predicate []
+    )
+  =
+  ()
+*)
+
 //---|
